src/tls/Format.KeyShareEntry.fsti
@@ -1,0 +1,29 @@
+module Format.KeyShareEntry
+
+open Format.NamedGroup
+
+module B = FStar.Bytes
+module LP = LowParse.SLow.Base
+module U32 = FStar.UInt32
+
+type keyShareEntry = {
+  group        : namedGroup; 
+  key_exchange : B.bytes; // (bs:B.bytes{1 <= B.length bs && B.length bs <= 65535});
+}
+
+inline_for_extraction
+val keyShareEntry_parser_kind_metadata : LP.parser_kind_metadata_t
+
+inline_for_extraction
+let keyShareEntry_parser_kind =
+  LP.strong_parser_kind 5 65539 keyShareEntry_parser_kind_metadata
+
+val keyShareEntry_parser: LP.parser keyShareEntry_parser_kind keyShareEntry
+
+inline_for_extraction
+val keyShareEntry_parser32: LP.parser32 keyShareEntry_parser
+
+val keyShareEntry_serializer: LP.serializer keyShareEntry_parser
+
+inline_for_extraction
+val keyShareEntry_serializer32: LP.serializer32 keyShareEntry_serializer
